Some updates in progs. A hole is left in floyd/globals_lemmas.v

progs/verif_nest2.v
@@ -1,1 +1,51 @@
-Write file: ~/Documents/vst-latest/vst/
+Require Import floyd.proofauto.
+Require Import progs.nest2.
+
+Local Open Scope logic.
+
+Definition get_spec :=
+ DECLARE _get
+  WITH v : reptype' t_struct_b, p : val
+  PRE  [] 
+        PROP ()
+        LOCAL(var _p t_struct_b p)
+        SEP(`(data_at Ews t_struct_b (repinj _ v) p))
+  POST [ tint ]
+         PROP() 
+         LOCAL (temp 1%positive (Vint (snd (snd v))))
+         SEP (`(data_at Ews t_struct_b (repinj _ v) p)).
+
+Definition update22 (i: int) (v: reptype' t_struct_b) : reptype' t_struct_b :=
+   (fst v, (fst (snd v), i)).
+
+Definition set_spec :=
+ DECLARE _set
+  WITH i : int, v : reptype' t_struct_b, p : val
+  PRE  [ _i OF tint ] 
+         PROP  ()
+         LOCAL (var _p t_struct_b p; 
+                temp _i (Vint i))
+         SEP   (`(data_at Ews t_struct_b (repinj _ v) p))
+  POST [ tvoid ]
+        `(data_at Ews t_struct_b (repinj _ (update22 i v)) p).
+
+Definition Vprog : varspecs := (_p, t_struct_b)::nil.
+
+Definition Gprog : funspecs := 
+    get_spec::set_spec::nil.
+
+Lemma body_get:  semax_body Vprog Gprog f_get get_spec.
+Proof.
+start_function.
+name i _i.
+forward.
+forward.
+Qed.
+
+Lemma body_set:  semax_body Vprog Gprog f_set set_spec.
+Proof.
+ start_function.
+name i_ _i.
+forward.
+forward.
+Qed.
